ulib/experimental/Steel.CStdInt.fsti
@@ -5,7 +5,11 @@ module I32 = FStar.Int32
 
 val size_t : Type0
 
-val size_v (x: size_t) : GTot nat
+val size_precond (x: nat) : Tot prop
+
+val size_v (x: size_t) : Pure nat // should be Ghost, but need Pure to implement alloc
+  (requires True)
+  (ensures (fun y -> size_precond y))
 
 val size_v_inj (x1 x2: size_t) : Lemma
   (size_v x1 == size_v x2 ==> x1 == x2)
@@ -15,6 +19,23 @@ val mk_size_t (x: U32.t) : Pure size_t
   (requires True)
   (ensures (fun y -> size_v y == U32.v x))
 
+val int_to_size_t (x: nat) : Ghost size_t
+  (requires (size_precond x))
+  (ensures (fun y -> size_v y == x))
+
+val size_precond_le (x y: nat) : Lemma
+  (requires (x <= y /\ size_precond y))
+  (ensures (size_precond x))
+  [SMTPat (size_precond x); SMTPat (size_precond y)]
+
+val size_add (x y: size_t) : Pure size_t
+  (requires (size_precond (size_v x + size_v y)))
+  (ensures (fun z -> size_v z == size_v x + size_v y))
+
+val size_sub (x y: size_t) : Pure size_t
+  (requires (size_v x >= size_v y))
+  (ensures (fun z -> size_v z == size_v x - size_v y))
+
 let zero_size : (zero_size: size_t { size_v zero_size == 0 }) = mk_size_t 0ul
 
 let one_size : (zero_size: size_t { size_v zero_size == 1 }) = mk_size_t 1ul
@@ -23,7 +44,7 @@ val ptrdiff_t : Type0
 
 module I32 = FStar.Int32
 
-val ptrdiff_v (x: ptrdiff_t) : GTot int
+val ptrdiff_v (x: ptrdiff_t) : Tot int // same remark as for size_v
 
 val ptrdiff_v_inj (x1 x2: ptrdiff_t) : Lemma
   (ptrdiff_v x1 == ptrdiff_v x2 ==> x1 == x2)
